Batteries/Data/Array/Pairwise.lean
@@ -20,7 +20,7 @@ that `as` is strictly sorted and `as.Pairwise (· ≤ ·)` asserts that `as` is 
 def Pairwise (R : α → α → Prop) (as : Array α) : Prop := as.toList.Pairwise R
 
 theorem pairwise_iff_get {as : Array α} : as.Pairwise R ↔
-    ∀ (i j : Fin as.size), i < j → R (as.get i) (as.get j) := by
+    ∀ (i j : Fin as.size), i < j → R (as.get i i.2) (as.get j j.2) := by
   unfold Pairwise; simp [List.pairwise_iff_get, getElem_fin_eq_getElem_toList]
 
 theorem pairwise_iff_getElem {as : Array α} : as.Pairwise R ↔
